Make the partial evaluator usable end-to-end
Now passes all the execution tests in test/c/. Some temporary hackiness
has been tolerated to bring it up to this pass rate, with the intent being
to have this suite passing as a baseline for further improvements and refactorings.

Some AI was used to identify and automatically fix failing tests, but also
significant manual refactoring was done to clean up the result. Where no
suitable primitive exists in the Rocq formalisation, we defer to the Sail_lib OCaml
implementations.

Assisted-by: Claude:Opus 4.8

src/lib/extraction/AbsBitvector.mli
@@ -55,7 +55,13 @@ module Dom :
 
   val leb : t -> t -> bool
 
+  val unknown_bit : bvset
+
+  val zwbv : bvset
+
   val _UU03b1_ : bvn -> bvset
+
+  val alpha : bvn -> bvset
 
   val lift_bitwise_gmap :
     (Three.ubit -> Three.ubit -> Three.ubit) -> (Big_int_Z.big_int,
