src/lib/extraction/Basics.ml
@@ -1,0 +1,5 @@
+
+(** val compose : ('a2 -> 'a3) -> ('a1 -> 'a2) -> 'a1 -> 'a3 **)
+
+let compose g f x =
+  g (f x)
