src/lib/extraction/Compare_dec.ml
@@ -1,0 +1,14 @@
+
+(** val le_lt_dec : Big_int_Z.big_int -> Big_int_Z.big_int -> bool **)
+
+let rec le_lt_dec = Big_int_Z.le_big_int
+
+(** val le_gt_dec : Big_int_Z.big_int -> Big_int_Z.big_int -> bool **)
+
+let le_gt_dec =
+  le_lt_dec
+
+(** val le_dec : Big_int_Z.big_int -> Big_int_Z.big_int -> bool **)
+
+let le_dec =
+  le_gt_dec
