src/lib/extraction/Interval.mli
@@ -47,6 +47,8 @@ module Dom :
 
   val alpha : Big_int_Z.big_int -> interval
 
+  val concrete : interval -> Big_int_Z.big_int option
+
   val compare_endpoints :
     (Big_int_Z.big_int -> Big_int_Z.big_int -> bool) -> Big_int_Z.big_int
     option -> Big_int_Z.big_int option -> bool
