src/lib/extraction/List0.mli
@@ -2,6 +2,8 @@ open Datatypes
 
 val tl : 'a1 list -> 'a1 list
 
+val nth_error : 'a1 list -> Big_int_Z.big_int -> 'a1 option
+
 val rev : 'a1 list -> 'a1 list
 
 val concat : 'a1 list list -> 'a1 list
