src/lib/extraction/PatternMatch.mli
@@ -13,7 +13,7 @@ open QArith_base
 open TypeAnnot
 
 type 'v binding =
-| Complete of value
+| Complete of 'v
 | Partial of (('v * Big_int_Z.big_int) * Big_int_Z.big_int) non_empty
 
 val combine_binding :
@@ -37,7 +37,7 @@ type 'v match_result =
 | Unmatched
 
 val merge_match_result :
-  value match_result -> value match_result -> value match_result
+  'a1 match_result -> 'a1 match_result -> 'a1 match_result
 
 val empty_bindings : 'a1 binding IdMap.t
 
