src/lib/extraction/PeanoNat.mli
@@ -1,6 +1,8 @@
 
 module Nat :
  sig
+  val add : Big_int_Z.big_int -> Big_int_Z.big_int -> Big_int_Z.big_int
+
   val sub : Big_int_Z.big_int -> Big_int_Z.big_int -> Big_int_Z.big_int
 
   val eqb : Big_int_Z.big_int -> Big_int_Z.big_int -> bool
