src/lib/extraction/TransferBitvectorInterval.mli
@@ -1,0 +1,291 @@
+open AbsBitvector
+open BinInt
+open BinNat
+open Bit
+open Datatypes
+open Interval
+open List0
+open ListDef
+open Nat0
+open PeanoNat
+open Specif
+open Base
+open Countable
+open Definitions
+open Fin_maps
+open Gmap
+open List_basics
+open Numbers
+
+module B :
+ sig
+  type bvset = AbsBitvector.Dom.bvset =
+  | Top
+  | Bvs of (Big_int_Z.big_int, Three.ubit list) gmap coq_sig
+
+  val bvset_rect :
+    'a1 -> ((Big_int_Z.big_int, Three.ubit list) gmap coq_sig -> 'a1) ->
+    bvset -> 'a1
+
+  val bvset_rec :
+    'a1 -> ((Big_int_Z.big_int, Three.ubit list) gmap coq_sig -> 'a1) ->
+    bvset -> 'a1
+
+  val to_bv_list : bvset -> Three.ubit list list option
+
+  type t = bvset
+
+  val top : bvset
+
+  val bot : t
+
+  val join_aux :
+    (Big_int_Z.big_int, Three.ubit list) gmap -> (Big_int_Z.big_int,
+    Three.ubit list) gmap -> (Big_int_Z.big_int, Three.ubit list) gmap
+
+  val join : t -> t -> t
+
+  val meet_aux :
+    (Big_int_Z.big_int, Three.ubit list) gmap -> (Big_int_Z.big_int,
+    Three.ubit list) gmap -> (Big_int_Z.big_int, Three.ubit list) gmap
+
+  val meet : t -> t -> t
+
+  val leb_aux :
+    (Big_int_Z.big_int, Three.ubit list) gmap -> (Big_int_Z.big_int,
+    Three.ubit list) gmap -> bool
+
+  val leb : t -> t -> bool
+
+  val unknown_bit : bvset
+
+  val zwbv : bvset
+
+  val _UU03b1_ : bvn -> bvset
+
+  val alpha : bvn -> bvset
+
+  val lift_bitwise_gmap :
+    (Three.ubit -> Three.ubit -> Three.ubit) -> (Big_int_Z.big_int,
+    Three.ubit list) gmap -> (Big_int_Z.big_int, Three.ubit list) gmap ->
+    (Big_int_Z.big_int, Three.ubit list) gmap
+
+  val lift_bitwise :
+    (Three.ubit -> Three.ubit -> Three.ubit) -> bvset -> bvset -> bvset
+
+  val coq_and : bvset -> bvset -> bvset
+
+  val coq_or : bvset -> bvset -> bvset
+
+  val xor : bvset -> bvset -> bvset
+
+  val not_gmap :
+    (Big_int_Z.big_int, Three.ubit list) gmap -> (Big_int_Z.big_int,
+    Three.ubit list) gmap
+
+  val not : bvset -> bvset
+
+  val add_gmap :
+    (Big_int_Z.big_int, Three.ubit list) gmap -> (Big_int_Z.big_int,
+    Three.ubit list) gmap -> (Big_int_Z.big_int, Three.ubit list) gmap
+
+  val add : bvset -> bvset -> bvset
+
+  val append_insert :
+    Three.ubit list -> Three.ubit list option -> Three.ubit list option
+
+  val append_gmap :
+    (Big_int_Z.big_int, Three.ubit list) gmap -> (Big_int_Z.big_int,
+    Three.ubit list) gmap -> (Big_int_Z.big_int, Three.ubit list) gmap
+
+  val append : bvset -> bvset -> bvset
+
+  val one_bits : Big_int_Z.big_int -> Three.ubit list
+
+  val negate_gmap :
+    (Big_int_Z.big_int, Three.ubit list) gmap -> (Big_int_Z.big_int,
+    Three.ubit list) gmap
+
+  val negate : bvset -> bvset
+
+  val sub : bvset -> bvset -> bvset
+
+  val slice_bits :
+    Three.ubit list -> Big_int_Z.big_int -> Big_int_Z.big_int -> Three.ubit
+    list
+
+  val slice_gmap :
+    (Big_int_Z.big_int, Three.ubit list) gmap -> Big_int_Z.big_int ->
+    Big_int_Z.big_int -> (Big_int_Z.big_int, Three.ubit list) gmap
+
+  val slice : bvset -> Big_int_Z.big_int -> Big_int_Z.big_int -> bvset
+ end
+
+module I :
+ sig
+  type endpoints =
+    (Big_int_Z.big_int option * Big_int_Z.big_int option) coq_sig
+
+  type interval = Dom.interval =
+  | Empty
+  | Ends of endpoints
+
+  val interval_rect : 'a1 -> (endpoints -> 'a1) -> interval -> 'a1
+
+  val interval_rec : 'a1 -> (endpoints -> 'a1) -> interval -> 'a1
+
+  type t = interval
+
+  val low : endpoints -> Big_int_Z.big_int option
+
+  val high : endpoints -> Big_int_Z.big_int option
+
+  val extend :
+    (Big_int_Z.big_int -> Big_int_Z.big_int -> bool) -> Big_int_Z.big_int
+    option -> Big_int_Z.big_int option -> Big_int_Z.big_int option
+
+  val join : interval -> interval -> interval
+
+  val meet : interval -> interval -> interval
+
+  val bot : interval
+
+  val top : interval
+
+  val low_leb : Big_int_Z.big_int option -> Big_int_Z.big_int option -> bool
+
+  val high_leb : Big_int_Z.big_int option -> Big_int_Z.big_int option -> bool
+
+  val leb : interval -> interval -> bool
+
+  val _UU03b1_ : Big_int_Z.big_int -> interval
+
+  val alpha : Big_int_Z.big_int -> interval
+
+  val concrete : interval -> Big_int_Z.big_int option
+
+  val compare_endpoints :
+    (Big_int_Z.big_int -> Big_int_Z.big_int -> bool) -> Big_int_Z.big_int
+    option -> Big_int_Z.big_int option -> bool
+
+  val lt : interval -> interval -> bool option
+
+  val gt : interval -> interval -> bool option
+
+  val lteq : interval -> interval -> bool option
+
+  val gteq : interval -> interval -> bool option
+
+  val negate_endpoints :
+    (Big_int_Z.big_int option * Big_int_Z.big_int option) ->
+    Big_int_Z.big_int option * Big_int_Z.big_int option
+
+  val negate : interval -> interval
+
+  val add_endpoints :
+    (Big_int_Z.big_int option * Big_int_Z.big_int option) ->
+    (Big_int_Z.big_int option * Big_int_Z.big_int option) ->
+    Big_int_Z.big_int option * Big_int_Z.big_int option
+
+  val add : interval -> interval -> interval
+
+  val sub : interval -> interval -> interval
+
+  val four_corner_endpoints :
+    (Big_int_Z.big_int -> Big_int_Z.big_int -> Big_int_Z.big_int) ->
+    (Big_int_Z.big_int option * Big_int_Z.big_int option) ->
+    (Big_int_Z.big_int option * Big_int_Z.big_int option) ->
+    Big_int_Z.big_int option * Big_int_Z.big_int option
+
+  val lift_binop :
+    (Big_int_Z.big_int -> Big_int_Z.big_int -> Big_int_Z.big_int) -> interval
+    -> interval -> interval
+
+  val mult : interval -> interval -> interval
+
+  val max_endpoints :
+    (Big_int_Z.big_int option * Big_int_Z.big_int option) ->
+    (Big_int_Z.big_int option * Big_int_Z.big_int option) ->
+    Big_int_Z.big_int option * Big_int_Z.big_int option
+
+  val max : interval -> interval -> interval
+
+  val min_endpoints :
+    (Big_int_Z.big_int option * Big_int_Z.big_int option) ->
+    (Big_int_Z.big_int option * Big_int_Z.big_int option) ->
+    Big_int_Z.big_int option * Big_int_Z.big_int option
+
+  val min : interval -> interval -> interval
+
+  val abs_endpoint :
+    (Big_int_Z.big_int option * Big_int_Z.big_int option) ->
+    Big_int_Z.big_int option * Big_int_Z.big_int option
+
+  val abs : interval -> interval
+
+  val tdiv : interval -> interval -> interval
+
+  val tmod : interval -> interval -> interval
+
+  val fdiv : interval -> interval -> interval
+
+  val fmod : interval -> interval -> interval
+
+  val ediv : interval -> interval -> interval
+
+  val emod : interval -> interval -> interval
+ end
+
+module Ops :
+ sig
+  val nonneg_top : I.t
+
+  val unsigned_lo : Three.ubit list -> Big_int_Z.big_int -> Big_int_Z.big_int
+
+  val unsigned_hi : Three.ubit list -> Big_int_Z.big_int -> Big_int_Z.big_int
+
+  val bits_unsigned_interval : Three.ubit list -> I.t
+
+  val unsigned : B.t -> I.t
+
+  val bits_signed_interval : Three.ubit list -> I.t
+
+  val signed : B.t -> I.t
+
+  val zeros_nat : Big_int_Z.big_int -> B.t
+
+  val ones_nat : Big_int_Z.big_int -> B.t
+
+  val nonneg_range :
+    I.t -> (Big_int_Z.big_int * Big_int_Z.big_int option) option
+
+  val zeros : Big_int_Z.big_int -> I.t -> B.t
+
+  val ones : Big_int_Z.big_int -> I.t -> B.t
+
+  val count_leading_B0 : Three.ubit list -> Big_int_Z.big_int
+
+  val count_until_B1 : Three.ubit list -> Big_int_Z.big_int
+
+  val bits_clz_interval : Three.ubit list -> I.t
+
+  val count_leading_zeros : B.t -> I.t
+
+  val bits_ctz_interval : Three.ubit list -> I.t
+
+  val count_trailing_zeros : B.t -> I.t
+
+  val zero_extend_one_width : Three.ubit list -> Big_int_Z.big_int -> B.t
+
+  val zero_extend_to_width : B.t -> Big_int_Z.big_int -> B.t
+
+  val zero_extend : Big_int_Z.big_int -> B.t -> I.t -> B.t
+
+  val sign_extend_one_width : Three.ubit list -> Big_int_Z.big_int -> B.t
+
+  val sign_extend_to_width : B.t -> Big_int_Z.big_int -> B.t
+
+  val sign_extend : Big_int_Z.big_int -> B.t -> I.t -> B.t
+
+  val bits_length : B.t -> I.t
+ end
