src/lib/extraction/fin_sets.mli
@@ -1,0 +1,5 @@
+open Basics
+open Datatypes
+open Base
+
+val set_size : ('a1, 'a2) coq_Elements -> 'a2 coq_Size
