test/sv/run_tests.py
@@ -34,6 +34,7 @@ skip_tests = {
     'simple_while', # loops
     'simple_while2', # loops
     'simple_while3', # loops
+    'repeat_loop', # loops
     'concurrency_interface_v2',
     'concurrency_interface_v2_var',
     'mini_builtins', # unsupported builtins
